it works

ProvenZk/Poseidon.lean
@@ -62,14 +62,12 @@ def perm (input_words : Vector F 3): Vector F 3 := Id.run do
 theorem test_vector_correct:
   perm vec![0,1,2] = vec![0x115cc0f5e7d690413df64c6b9662e9cf2a3617f2743245519e19607a4417189a, 0x0fca49b798923ab0239de1c9e7a4a9a2210312b6a2f616d18b5a87f9b628ae29, 0x0e7ae82e40091e63cbd4f16a6d16310b3729d4b6e138fcf54110e2867045a30c] := by eq_refl
 
--- def full_round_cps (state : Array F) (k : Array F -> α) (round : Nat): α :=
+lemma vector_3_decomp [Inhabited α] (v : Vector α 3): v = vec![v[0]!, v[1]!, v[2]!] := by
+  sorry
 
-
--- def perm_cps (state : Array F)
-
-def full_rounds_step_1 (input_words : Vector F 3) (round_constants_counter : Nat) (num_rounds : Nat): Id (MProd Nat (Vector F 3)) := do
-  let mut round_constants_counter := round_constants_counter
-  let mut state_words := input_words
+def full_rounds_step_1 (inp : MProd Nat (Vector F 3)) (num_rounds : Nat): Id (MProd Nat (Vector F 3)) := do
+  let mut round_constants_counter := inp.1
+  let mut state_words := inp.2
   for r in [0:num_rounds] do
     for i in [0:t] do
       state_words := state_words.set i (state_words[i]! + round_constants_field[round_constants_counter]!)
@@ -92,9 +90,188 @@ def full_round_step_1 (inp : MProd Nat (Vector F 3)): Id (MProd Nat (Vector F 3)
   state_words := (MDS_matrix_field.mul state_words_vec).to_vector
   ⟨round_constants_counter, state_words⟩
 
-def full_rounds_step_2 (input_words : Vector F 3) (round_constants_counter : Nat) (num_rounds : Nat): Id (MProd Nat (Vector F 3)) := do
-  let mut round_constants_counter := round_constants_counter
-  let mut state_words := input_words
+def partial_round_step_1 (inp : MProd Nat (Vector F 3)): Id (MProd Nat (Vector F 3)) := do
+  let mut round_constants_counter := inp.1
+  let mut state_words := inp.2
+  for i in [0:t] do
+    state_words := state_words.set i (state_words[i]! + round_constants_field[round_constants_counter]!)
+    round_constants_counter := round_constants_counter + 1
+  state_words := state_words.set 0 (state_words[0]! ^ 5)
+  let state_words_vec := Matrix.column_from_vector state_words
+  state_words := (MDS_matrix_field.mul state_words_vec).to_vector
+  ⟨round_constants_counter, state_words⟩
+
+def add_constants_step_1 (inp : MProd Nat (Vector F 3)): Id (MProd Nat (Vector F 3)) := do
+  let mut round_constants_counter := inp.1
+  let mut state_words := inp.2
+  for i in [0:t] do
+    state_words := state_words.set i (state_words[i]! + round_constants_field[round_constants_counter]!)
+    round_constants_counter := round_constants_counter + 1
+  ⟨round_constants_counter, state_words⟩
+
+def add_constants_step_2 (inp : MProd Nat (Vector F 3)): MProd Nat (Vector F 3) :=
+  ⟨inp.1 + 3, vec![
+    inp.2[0] + round_constants_field[inp.1]!,
+    inp.2[1] + round_constants_field[inp.1.succ]!,
+    inp.2[2] + round_constants_field[inp.1.succ.succ]!
+  ]⟩
+
+theorem add_constants_step_2_go {inp : MProd Nat (Vector F 3)}: add_constants_step_1 inp = add_constants_step_2 inp := by
+  unfold add_constants_step_1
+  unfold add_constants_step_2
+  simp
+  (
+    split; rename_i rc sw h;
+    have : sw = (MProd.mk rc sw).2 := by rfl
+    rw [this]; clear this;
+    have : rc = (MProd.mk rc sw).1 := by rfl
+    rw [this]; clear this;
+    have : MProd.mk (MProd.mk rc sw).1 sw = MProd.mk rc sw := by rfl
+    rw [this]; clear this;
+    rw [←h]; clear rc sw h;
+  )
+  simp [forIn, Std.Range.forIn, Std.Range.forIn.loop]
+  rw [vector_3_decomp inp.2]
+  rfl
+
+def full_round_step_2 (inp : MProd Nat (Vector F 3)): Id (MProd Nat (Vector F 3)) := do
+  let mut round_constants_counter := inp.1
+  let mut state_words := inp.2
+  match add_constants_step_1 inp with
+  | ⟨rc, sw⟩ => do
+    round_constants_counter := rc
+    state_words := sw
+  for i in [0:t] do
+    state_words := state_words.set i (state_words[i]! ^ 5)
+  let state_words_vec := Matrix.column_from_vector state_words
+  state_words := (MDS_matrix_field.mul state_words_vec).to_vector
+  ⟨round_constants_counter, state_words⟩
+
+theorem full_round_step_2_go {inp : MProd Nat (Vector F 3)}:
+  full_round_step_1 inp = full_round_step_2 inp := by
+  unfold full_round_step_1
+  unfold full_round_step_2
+  congr
+
+
+def partial_round_step_2 (inp : MProd Nat (Vector F 3)): Id (MProd Nat (Vector F 3)) := do
+  let mut round_constants_counter := inp.1
+  let mut state_words := inp.2
+  match add_constants_step_1 inp with
+  | ⟨rc, sw⟩ => do
+    round_constants_counter := rc
+    state_words := sw
+  state_words := state_words.set 0 (state_words[0]! ^ 5)
+  let state_words_vec := Matrix.column_from_vector state_words
+  state_words := (MDS_matrix_field.mul state_words_vec).to_vector
+  ⟨round_constants_counter, state_words⟩
+
+theorem partial_round_step_2_go {inp : MProd Nat (Vector F 3)}:
+  partial_round_step_1 inp = partial_round_step_2 inp := by
+  unfold partial_round_step_1
+  unfold partial_round_step_2
+  congr
+
+
+def sbox_all_step_1 (inp : Vector F 3): Id (Vector F 3) := do
+  let mut state_words := inp
+  for i in [0:t] do
+    state_words := state_words.set i (state_words[i]! ^ 5)
+  state_words
+
+def sbox_all_step_2 (inp : Vector F 3): Vector F 3 :=
+  vec![inp[0] ^ 5, inp[1] ^ 5, inp[2] ^ 5]
+
+theorem sbox_all_step_2_go {inp : Vector F 3}:
+  sbox_all_step_1 inp = sbox_all_step_2 inp := by
+  unfold sbox_all_step_1
+  unfold sbox_all_step_2
+  simp [forIn, Std.Range.forIn, Std.Range.forIn.loop]
+  rw [vector_3_decomp inp]
+  rfl
+
+def full_round_step_3 (inp : MProd Nat (Vector F 3)): Id (MProd Nat (Vector F 3)) := do
+  let mut round_constants_counter := inp.1
+  let mut state_words := inp.2
+  match add_constants_step_1 inp with
+  | ⟨rc, sw⟩ => do
+    round_constants_counter := rc
+    state_words := sw
+  state_words := (← sbox_all_step_1 state_words)
+  let state_words_vec := Matrix.column_from_vector state_words
+  state_words := (MDS_matrix_field.mul state_words_vec).to_vector
+  ⟨round_constants_counter, state_words⟩
+
+theorem full_round_step_3_go {inp : MProd Nat (Vector F 3)}:
+  full_round_step_2 inp = full_round_step_3 inp := by
+  unfold full_round_step_2
+  unfold full_round_step_3
+  simp
+  (
+    split; rename_i rc sw h;
+    have : sw = (MProd.mk rc sw).2 := by rfl
+    rw [this]; clear this;
+    have : rc = (MProd.mk rc sw).1 := by rfl
+    rw [this]; clear this;
+    have : MProd.mk (MProd.mk rc sw).1 sw = MProd.mk rc sw := by rfl
+    rw [this]; clear this;
+    rw [←h]; clear rc sw h;
+  )
+  congr
+
+def mds_matmul (S : Vector F 3) : Vector F 3 :=
+  let smat := Matrix.column_from_vector S
+  let rmat := MDS_matrix_field.mul smat
+  vec![rmat 0 0, rmat 1 0, rmat 2 0]
+
+def full_round (S C: Vector F 3) : Vector F 3 :=
+  mds_matmul vec![(S[0] + C[0]) ^ 5, (S[1] + C[1]) ^ 5, (S[2] + C[2]) ^ 5]
+
+def partial_round (S C: Vector F 3) : Vector F 3 :=
+  mds_matmul vec![(S[0] + C[0]) ^ 5, S[1] + C[1], S[2] + C[2]]
+
+def full_round_step_4 (const_counter: Nat) (words: Vector F 3): (Vector F 3) :=
+  full_round words vec![
+    round_constants_field[const_counter]!,
+    round_constants_field[const_counter.succ]!,
+    round_constants_field[const_counter.succ.succ]!
+  ]
+
+theorem full_round_step_4_go {inp : MProd Nat (Vector F 3)}: full_round_step_3 inp = ⟨inp.1.succ.succ.succ, full_round_step_4 inp.1 inp.2⟩ := by
+  unfold full_round_step_3
+  unfold full_round_step_4
+  simp
+  (
+    split; rename_i rc sw h;
+    have : sw = (MProd.mk rc sw).2 := by rfl
+    rw [this]; clear this;
+    have : rc = (MProd.mk rc sw).1 := by rfl
+    rw [this]; clear this;
+    have : MProd.mk (MProd.mk rc sw).1 sw = MProd.mk rc sw := by rfl
+    rw [this]; clear this;
+    rw [←h]; clear rc sw h;
+  )
+  rw [add_constants_step_2_go, sbox_all_step_2_go]
+  rfl
+
+def partial_round_step_3 (const_counter: Nat) (words: Vector F 3): (Vector F 3) :=
+  partial_round words vec![
+    round_constants_field[const_counter]!,
+    round_constants_field[const_counter.succ]!,
+    round_constants_field[const_counter.succ.succ]!
+  ]
+
+theorem partial_round_step_3_go {inp : MProd Nat (Vector F 3)}:
+  partial_round_step_2 inp = ⟨inp.1.succ.succ.succ, partial_round_step_3 inp.1 inp.2⟩ := by
+  unfold partial_round_step_2
+  unfold partial_round_step_3
+  simp
+  rw [add_constants_step_2_go]
+  congr
+
+def full_rounds_step_2 (inp : MProd Nat (Vector F 3)) (num_rounds : Nat): Id (MProd Nat (Vector F 3)) := do
+  let mut round_constants_counter := inp.1
+  let mut state_words := inp.2
   for r in [0:num_rounds] do
     match full_round_step_1 ⟨round_constants_counter, state_words⟩ with
     | ⟨rc, sw⟩ => do
@@ -102,8 +279,8 @@ def full_rounds_step_2 (input_words : Vector F 3) (round_constants_counter : Nat
       state_words := sw
   ⟨round_constants_counter, state_words⟩
 
-lemma full_rounds_step_2_go {inp : Vector F 3} { rcc num_rounds : Nat}:
-  full_rounds_step_1 inp rcc num_rounds = full_rounds_step_2 inp rcc num_rounds := by
+lemma full_rounds_step_2_go {inp : MProd Nat (Vector F 3)} { num_rounds : Nat}:
+  full_rounds_step_1 inp num_rounds = full_rounds_step_2 inp num_rounds := by
   unfold full_rounds_step_1
   unfold full_rounds_step_2
   simp
@@ -132,9 +309,34 @@ lemma full_rounds_step_2_go {inp : Vector F 3} { rcc num_rounds : Nat}:
   rw [this]; clear this;
   rw [←h];
 
-def partial_rounds_step_1 (input_words : Vector F 3) (round_constants_counter : Nat) (num_rounds : Nat): Id (MProd Nat (Vector F 3)) := do
-  let mut round_constants_counter := round_constants_counter
-  let mut state_words := input_words
+def full_rounds_step_3 (inp : MProd Nat (Vector F 3)) (num_rounds : Nat): Id (MProd Nat (Vector F 3)) := do
+  let mut round_constants_counter := inp.1
+  let mut state_words := inp.2
+  for r in [0:num_rounds] do
+    let consts := vec![
+      round_constants_field[round_constants_counter]!,
+      round_constants_field[round_constants_counter.succ]!,
+      round_constants_field[round_constants_counter.succ.succ]!
+    ]
+    state_words := full_round state_words consts
+    round_constants_counter := round_constants_counter.succ.succ.succ
+  ⟨round_constants_counter, state_words⟩
+
+theorem full_rounds_step_3_go (inp : MProd Nat (Vector F 3)) (num_rounds : Nat):
+  full_rounds_step_2 inp num_rounds = full_rounds_step_3 inp num_rounds := by
+  unfold full_rounds_step_2
+  unfold full_rounds_step_3
+  simp
+  split; rename_i h; rw [←h]; clear h;
+  split; rename_i h; rw [←h]; clear h;
+  apply congrArg
+  funext
+  rw [full_round_step_2_go, full_round_step_3_go, full_round_step_4_go]
+  congr
+
+def partial_rounds_step_1 (inp : MProd Nat (Vector F 3)) (num_rounds : Nat): Id (MProd Nat (Vector F 3)) := do
+  let mut round_constants_counter := inp.1
+  let mut state_words := inp.2
   for r in [0:num_rounds] do
     for i in [0:t] do
       state_words := state_words.set i (state_words[i]! + round_constants_field[round_constants_counter]!)
@@ -144,31 +346,70 @@ def partial_rounds_step_1 (input_words : Vector F 3) (round_constants_counter : 
     state_words := (MDS_matrix_field.mul state_words_vec).to_vector
   ⟨round_constants_counter, state_words⟩
 
+def partial_rounds_step_2 (inp : MProd Nat (Vector F 3)) (num_rounds : Nat): Id (MProd Nat (Vector F 3)) := do
+  let mut round_constants_counter := inp.1
+  let mut state_words := inp.2
+  for r in [0:num_rounds] do
+    match partial_round_step_1 ⟨round_constants_counter, state_words⟩ with
+    | ⟨rc, sw⟩ => do
+      round_constants_counter := rc
+      state_words := sw
+  ⟨round_constants_counter, state_words⟩
+
+theorem partial_rounds_step_2_go {inp: MProd Nat (Vector F 3)} {num_rounds: Nat}:
+  partial_rounds_step_1 inp num_rounds = partial_rounds_step_2 inp num_rounds := by
+  unfold partial_rounds_step_1
+  unfold partial_rounds_step_2
+  simp
+  split; rename_i h; rw [←h]; clear h;
+  split; rename_i h; rw [←h]; clear h;
+  congr
+
+def partial_rounds_step_3 (inp : MProd Nat (Vector F 3)) (num_rounds : Nat): Id (MProd Nat (Vector F 3)) := do
+  let mut round_constants_counter := inp.1
+  let mut state_words := inp.2
+  for r in [0:num_rounds] do
+    let consts := vec![
+      round_constants_field[round_constants_counter]!,
+      round_constants_field[round_constants_counter.succ]!,
+      round_constants_field[round_constants_counter.succ.succ]!
+    ]
+    state_words := partial_round state_words consts
+    round_constants_counter := round_constants_counter.succ.succ.succ
+  ⟨round_constants_counter, state_words⟩
+
+theorem partial_rounds_step_3_go (inp : MProd Nat (Vector F 3)) (num_rounds : Nat):
+  partial_rounds_step_2 inp num_rounds = partial_rounds_step_3 inp num_rounds := by
+  unfold partial_rounds_step_2
+  unfold partial_rounds_step_3
+  simp
+  split; rename_i h; rw [←h]; clear h;
+  split; rename_i h; rw [←h]; clear h;
+  apply congrArg
+  funext
+  rw [partial_round_step_2_go, partial_round_step_3_go]
+  congr
+
+
 def step_1 (input_words : Vector F 3): Vector F 3 := Id.run do
   let R_f := R_F / 2
   let mut round_constants_counter := 0
   let mut state_words := input_words
-  match full_rounds_step_1 state_words round_constants_counter R_f with
+  match full_rounds_step_1 (MProd.mk round_constants_counter state_words) R_f with
   | ⟨rc, sw⟩ => do
     round_constants_counter := rc
     state_words := sw
 
-  for r in [0:R_P] do
-    for i in [0:t] do
-      state_words := state_words.set i (state_words[i]! + round_constants_field[round_constants_counter]!)
-      round_constants_counter := round_constants_counter + 1
-    state_words := state_words.set 0 (state_words[0]! ^ 5)
-    let state_words_vec := Matrix.column_from_vector state_words
-    state_words := (MDS_matrix_field.mul state_words_vec).to_vector
+  match partial_rounds_step_1 (MProd.mk round_constants_counter state_words) R_P with
+  | ⟨rc, sw⟩ => do
+    round_constants_counter := rc
+    state_words := sw
 
-  for r in [0:R_f] do
-    for i in [0:t] do
-      state_words := state_words.set i (state_words[i]! + round_constants_field[round_constants_counter]!)
-      round_constants_counter := round_constants_counter + 1
-    for i in [0:t] do
-      state_words := state_words.set i (state_words[i]! ^ 5)
-    let state_words_vec := Matrix.column_from_vector state_words
-    state_words := (MDS_matrix_field.mul state_words_vec).to_vector
+  match full_rounds_step_1 (MProd.mk round_constants_counter state_words) R_f with
+  | ⟨rc, sw⟩ => do
+    round_constants_counter := rc
+    state_words := sw
+
   state_words
 
 lemma step1_go {input_words : Vector F 3}: perm input_words = step_1 input_words := by
@@ -177,133 +418,92 @@ lemma step1_go {input_words : Vector F 3}: perm input_words = step_1 input_words
   simp [Id.run]
   unfold full_rounds_step_1
   simp
-  split
-  rename_i h
-  rw [h]
-
-def step_2 (input_words : Vector F 3): Vector F 3 := Id.run do
-  let R_f := R_F / 2
-  let mut round_constants_counter := 0
-  let mut state_words := input_words
-  match full_rounds_step_1 state_words round_constants_counter R_f with
-  | ⟨rc, sw⟩ => do
-    round_constants_counter := rc
-    state_words := sw
-
-  for r in [0:R_P] do
-    for i in [0:t] do
-      state_words := state_words.set i (state_words[i]! + round_constants_field[round_constants_counter]!)
-      round_constants_counter := round_constants_counter + 1
-    state_words := state_words.set 0 (state_words[0]! ^ 5)
-    let state_words_vec := Matrix.column_from_vector state_words
-    state_words := (MDS_matrix_field.mul state_words_vec).to_vector
-
-  match full_rounds_step_1 state_words round_constants_counter R_f with
-  | ⟨rc, sw⟩ => do
-    round_constants_counter := rc
-    state_words := sw
-  state_words
-
--- lemma un_project {a : Id (MProd Nat (Vector F 3))} : (match a with | ⟨x, y⟩ => ⟨x, y⟩) = a := by
---   cases a
---   rfl
-
-lemma un_project {a : MProd α β} : ⟨a.1, a.2⟩ = a := by
-  cases a
-  rfl
-
-lemma un_match_snd {a : Id (MProd α β)} : (match a with | ⟨_, y⟩ => y) = a.2 := by
-  cases a
-  rfl
-
-
-def step_2_go (input_words : Vector F 3): step_1 input_words = step_2 input_words := by
-  unfold step_1
-  unfold step_2
-  simp [Id.run]
-  split
-  simp [full_rounds_step_1, un_project]
-  split
-  rename_i rc sw h
-  have : sw = (MProd.mk rc sw).2 := by rfl
-  rw [this]
-  rw [←h]
-  clear this rc sw h
-  apply congrArg
-  split
-  rename_i h
-  rw [←h]
-
-  -- simp [un_match]
-
-
-def step_3 (input_words : Vector F 3): Vector F 3 := Id.run do
-  let R_f := R_F / 2
-  let mut round_constants_counter := 0
-  let mut state_words := input_words
-  match full_rounds_step_1 state_words round_constants_counter R_f with
-  | ⟨rc, sw⟩ => do
-    round_constants_counter := rc
-    state_words := sw
-
-  match partial_rounds_step_1 state_words round_constants_counter R_P with
-  | ⟨rc, sw⟩ => do
-    round_constants_counter := rc
-    state_words := sw
-
-  match full_rounds_step_1 state_words round_constants_counter R_f with
-  | ⟨rc, sw⟩ => do
-    round_constants_counter := rc
-    state_words := sw
-  state_words
-
-lemma step_3_go {input_words : Vector F 3}: step_2 input_words = step_3 input_words := by
-  unfold step_2
-  unfold step_3
-  simp [Id.run]
-  split
-  split; rename_i rc sw h
-  have : sw = (MProd.mk rc sw).2 := by rfl
-  rw [this]
-  rw [←h]
-  clear this rc sw h
-  split; rename_i rc' sw' h'
-  split; rename_i rc'' sw'' h''
-  have : sw'' = (MProd.mk rc'' sw'').2 := by rfl
-  rw [this]
-  rw [←h'']
-  clear this rc'' sw'' h''
-  have : sw' = (MProd.mk rc' sw').2 := by rfl
-  rw [this]
-  clear this
-  have : rc' = (MProd.mk rc' sw').1 := by rfl
-  rw [this]
-  clear this
-  have : MProd.mk (MProd.mk rc' sw').1 sw' = MProd.mk rc' sw' := by rfl
-  rw [this]
-  rw [←h']
-  clear this rc' sw' h'
+  split; rename_i h; rw [←h]; clear h;
+  split; rename_i h; rw [←h]; clear h;
+  split; rename_i h; rw [←h]; clear h;
+  (
+    split
+    rename_i rc sw h
+    have : sw = (MProd.mk rc sw).2 := by rfl
+    rw [this, ←h]
+    clear this rc sw h
+  )
+  split; rename_i h; rw [←h]; clear h;
   apply congrArg
   apply congr
   {
+    apply congrArg
+    unfold partial_rounds_step_1
+    simp
+    split; rename_i h; rw [←h]; clear h;
+    have un_project : ∀ {α β} {a : MProd α β}, MProd.mk a.fst a.snd = a := by intro α β a; cases a; rfl
+    rw [un_project]
     apply congr
     {
       apply congrArg
-      apply congrArg
-      unfold partial_rounds_step_1
-      simp
-      split; rename_i h
-      rw [h]
+      rw [un_project]
+      split; rename_i h; rw [←h]
     }
-    {
-      apply congrArg
-      unfold partial_rounds_step_1
-      simp
-      split; rename_i h
-      rw [h]
-
-    }
+    { rfl }
   }
-  eq_refl
+  { rfl }
 
-end Poseidon
+
+def readable_perm (input_words : Vector F 3): Vector F 3 := Id.run do
+  let R_f := R_F / 2
+  let mut round_constants_counter := 0
+  let mut state_words := input_words
+  for r in [0:R_f] do
+    let consts := vec![
+      round_constants_field[round_constants_counter]!,
+      round_constants_field[round_constants_counter.succ]!,
+      round_constants_field[round_constants_counter.succ.succ]!
+    ]
+    state_words := full_round state_words consts
+    round_constants_counter := round_constants_counter.succ.succ.succ
+
+  for r in [0:R_P] do
+    let consts := vec![
+      round_constants_field[round_constants_counter]!,
+      round_constants_field[round_constants_counter.succ]!,
+      round_constants_field[round_constants_counter.succ.succ]!
+    ]
+    state_words := partial_round state_words consts
+    round_constants_counter := round_constants_counter.succ.succ.succ
+
+  for r in [0:R_f] do
+    let consts := vec![
+      round_constants_field[round_constants_counter]!,
+      round_constants_field[round_constants_counter.succ]!,
+      round_constants_field[round_constants_counter.succ.succ]!
+    ]
+    state_words := full_round state_words consts
+    round_constants_counter := round_constants_counter.succ.succ.succ
+  state_words
+
+theorem readable_perm_go (input_words : Vector F 3): perm input_words = readable_perm input_words := by
+  rw [step1_go]
+  unfold step_1
+  unfold readable_perm
+  simp [Id.run]
+  split; rename_i h; rw [←h]; clear h;
+  split; rename_i h; rw [←h]; clear h;
+  (
+    split
+    rename_i rc sw h
+    have : sw = (MProd.mk rc sw).2 := by rfl
+    rw [this, ←h]
+    clear this rc sw h
+  )
+  rw [full_rounds_step_2_go, full_rounds_step_3_go]
+  rw [full_rounds_step_2_go, full_rounds_step_3_go]
+  rw [partial_rounds_step_2_go, partial_rounds_step_3_go]
+  unfold full_rounds_step_3
+  unfold partial_rounds_step_3
+  simp
+  split; rename_i h; rw [←h]; clear h;
+  split; rename_i h; rw [←h]; clear h;
+  split; rename_i h; rw [←h]; clear h;
+  congr
+
+
