ProvenZk/PoseidonCorrectness.lean
@@ -22,500 +22,269 @@ lemma sbox_uncps (A : F) (k : F -> Prop): sbox A k = k (A ^ 5) := by
   simp_arith
   apply fin_mod _
 
-def mds_matmul (S : Vector F 3) : Vector F 3 :=
-  let smat := Matrix.column_from_vector S
-  let rmat := Poseidon.MDS_matrix_field.mul smat
-  vec![rmat 0 0, rmat 1 0, rmat 2 0]
 
-lemma vec_eq (a b : α) (t s : Vector α n) : a = b -> t = s -> a ::ᵥ t = b ::ᵥ s := by
+lemma mds_uncps (S : Vector F 3) (k : Vector F 3 -> Prop): mds_3 S k = k (Poseidon.mds_matmul S) := by
+  sorry
+
+lemma full_round_uncps (S C: Vector F 3) (k : Vector F 3 -> Prop): fullRound_3_3 S C k = k (Poseidon.full_round S C) := by
+  conv => lhs; simp [fullRound_3_3, Gates.add, sbox_uncps, mds_uncps]
+
+lemma half_round_uncps (S C: Vector F 3) (k : Vector F 3 -> Prop): halfRound_3_3 S C k = k (Poseidon.partial_round S C) := by
+  conv => lhs; simp [halfRound_3_3, Gates.add, sbox_uncps, mds_uncps]
+
+lemma iff_to_eq {α} {a b: α} {k : α -> Prop }: a = b -> (k a ↔ k b) := by intro eq; rw [eq]
+
+
+-- lemma full_rounds_1_uncps {S: Vector F 3} {k: Vector F 3 -> Prop}:
+--   full_rounds_cps' S 0 4 k = k (Poseidon.full_rounds_step_3 ⟨0, S⟩ 4).2 := by
+--   simp [full_rounds_cps', full_round_uncps, round_constants', Poseidon.round_constants_field, getElem!]
+--   apply iff_to_eq
+--   unfold Poseidon.full_rounds_step_3
+--   simp
+--   split; rename_i h; rw [←h]; clear h
+--   simp [forIn, Std.Range.forIn, Std.Range.forIn.loop, Poseidon.round_constants_field]
+--   simp [getElem!]
+
+-- lemma full_rounds_2_uncps {S : Vector F 3} {k : Vector F 3 -> Prop}:
+--   full_rounds_cps' S 183 4 k = k (Poseidon.full_rounds_step_3 ⟨183, S⟩ 4).2 := by
+--   simp [full_rounds_cps', full_round_uncps, round_constants', Poseidon.round_constants_field, getElem!]
+--   apply iff_to_eq
+--   unfold Poseidon.full_rounds_step_3
+--   simp
+--   split; rename_i h; rw [←h]; clear h
+--   simp [forIn, Std.Range.forIn, Std.Range.forIn.loop, Poseidon.round_constants_field]
+--   simp [getElem!]
+
+lemma full_rounds_cps'_tear (state: Vector F 3) (init_const: Nat) (round_count: Nat) (k : Vector F 3 -> Prop):
+    full_rounds_cps' (state: Vector F 3) (init_const) (round_count.succ) k =
+    full_rounds_cps' (Poseidon.full_round state (round_constants' init_const)) init_const.succ.succ.succ round_count k := by
+  simp [full_rounds_cps']
+  rw [full_round_uncps]
+
+lemma half_rounds_cps'_tear (state: Vector F 3) (init_const: Nat) (round_count: Nat) (k : Vector F 3 -> Prop):
+    half_rounds_cps' (state: Vector F 3) (init_const) (round_count.succ) k =
+    half_rounds_cps' (Poseidon.partial_round state (round_constants' init_const)) init_const.succ.succ.succ round_count k := by
+  simp [half_rounds_cps']
+  rw [half_round_uncps]
+
+lemma loop_invariant [Monad m] {stop start fuel: Nat} {s : α} {f : Nat -> α -> m (ForInStep α)}:
+  (∀i1 i2 a, f i1 a = f i2 a) ->
+  Std.Range.forIn.loop f fuel start.succ stop.succ 1 s = Std.Range.forIn.loop f fuel start stop 1 s := by
+  intro h
+  induction fuel generalizing start stop s with
+  | zero =>
+    simp [Std.Range.forIn.loop]
+  | succ fuel ih =>
+    simp [Std.Range.forIn.loop]
+    split
+    {
+      have : stop ≤ start := by
+        rw [←Nat.succ_le_succ_iff]
+        assumption
+      simp [this]
+    }
+    {
+      have : ¬ stop ≤ start := by
+        rw [←Nat.succ_le_succ_iff]
+        assumption
+      simp [this]
+      have : f start s = f start.succ s := by
+        apply h
+      simp [this]
+      unfold bind
+      apply congrArg
+      funext
+      split
+      {rfl}
+      {rw [ih]}
+    }
+
+lemma full_round_step_3_tear {inp : MProd Nat (Vector F 3)} {count}:
+  Poseidon.full_rounds_step_3 inp count.succ =
+  Poseidon.full_rounds_step_3 ⟨inp.1.succ.succ.succ, Poseidon.full_round inp.2 (round_constants' inp.1)⟩ count := by
+  conv =>
+    lhs
+    simp [Poseidon.full_rounds_step_3, forIn, Std.Range.forIn, Std.Range.forIn.loop]
+  conv =>
+    rhs
+    simp [Poseidon.full_rounds_step_3, forIn, Std.Range.forIn, Std.Range.forIn.loop, round_constants']
+  split; rename_i h; rw [←h]; clear h
+  split; rename_i h; rw [←h]; clear h
+  simp [loop_invariant]
+
+lemma full_round_const_count {inp : MProd Nat (Vector F 3)} {count}:
+  (Poseidon.full_rounds_step_3 inp count).1 = inp.1 + count * 3 := by
+  induction count generalizing inp with
+  | zero =>
+    simp [Poseidon.full_rounds_step_3, forIn, Std.Range.forIn, Std.Range.forIn.loop]
+  | succ count ih =>
+    rw [full_round_step_3_tear, ih]
+    simp
+    linarith
+
+lemma partial_round_step_3_tear {inp : MProd Nat (Vector F 3)} {count}:
+  Poseidon.partial_rounds_step_3 inp count.succ =
+  Poseidon.partial_rounds_step_3 ⟨inp.1.succ.succ.succ, Poseidon.partial_round inp.2 (round_constants' inp.1)⟩ count := by
+  conv =>
+    lhs
+    simp [Poseidon.partial_rounds_step_3, forIn, Std.Range.forIn, Std.Range.forIn.loop]
+  conv =>
+    rhs
+    simp [Poseidon.partial_rounds_step_3, forIn, Std.Range.forIn, Std.Range.forIn.loop, round_constants']
+  split; rename_i h; rw [←h]; clear h
+  split; rename_i h; rw [←h]; clear h
+  simp [loop_invariant]
+
+lemma partial_round_const_count {inp : MProd Nat (Vector F 3)} {count}:
+  (Poseidon.partial_rounds_step_3 inp count).1 = inp.1 + count * 3 := by
+  induction count generalizing inp with
+  | zero =>
+    simp [Poseidon.partial_rounds_step_3, forIn, Std.Range.forIn, Std.Range.forIn.loop]
+  | succ count ih =>
+    rw [partial_round_step_3_tear, ih]
+    simp
+    linarith
+
+lemma partial_rounds_uncps {S : Vector F 3} {start count : Nat} {k : Vector F 3 -> Prop}:
+  half_rounds_cps' S start count k = k (Poseidon.partial_rounds_step_3 ⟨start, S⟩ count).2 := by
+  induction count generalizing start S with
+  | zero =>
+    simp [half_rounds_cps', Poseidon.partial_rounds_step_3, forIn, Std.Range.forIn, Std.Range.forIn.loop]
+  | succ count ih =>
+    rw [partial_round_step_3_tear]
+    rw [half_rounds_cps'_tear]
+    apply ih
+
+lemma full_rounds_uncps {S : Vector F 3} {start count : Nat} {k : Vector F 3 -> Prop}:
+  full_rounds_cps' S start count k = k (Poseidon.full_rounds_step_3 ⟨start, S⟩ count).2 := by
+  induction count generalizing start S with
+  | zero =>
+    simp [full_rounds_cps', Poseidon.full_rounds_step_3, forIn, Std.Range.forIn, Std.Range.forIn.loop]
+  | succ count ih =>
+    rw [full_round_step_3_tear]
+    rw [full_rounds_cps'_tear]
+    apply ih
+
+def step_2 (input_words : Vector F 3): Vector F 3 := Id.run do
+  let R_f := Poseidon.R_F / 2
+  let mut round_constants_counter := 0
+  let mut state_words := input_words
+  match Poseidon.full_rounds_step_3 (MProd.mk round_constants_counter state_words) R_f with
+  | ⟨rc, sw⟩ => do
+    round_constants_counter := 12
+    state_words := sw
+
+  match Poseidon.partial_rounds_step_3 (MProd.mk round_constants_counter state_words) Poseidon.R_P with
+  | ⟨rc, sw⟩ => do
+    round_constants_counter := 183
+    state_words := sw
+
+  match Poseidon.full_rounds_step_3 (MProd.mk round_constants_counter state_words) R_f with
+  | ⟨rc, sw⟩ => do
+    round_constants_counter := 195
+    state_words := sw
+
+  state_words
+
+lemma step_2_go {input_words : Vector F 3}: Poseidon.step_1 input_words = step_2 input_words := by
+  unfold Poseidon.step_1
+  simp
+  simp [Poseidon.full_rounds_step_2_go, Poseidon.partial_rounds_step_2_go]
+  simp [Poseidon.full_rounds_step_3_go, Poseidon.partial_rounds_step_3_go]
+  simp [Id.run]
+  split; rename_i h; rw [←h]; clear h
+  split; rename_i h; rw [←h]; clear h
+  (
+    split
+    rename_i rc sw h
+    have : sw = (MProd.mk rc sw).2 := by rfl
+    rw [this, ←h]
+    clear this rc sw h
+  )
+  have : ∀ (a : Id (MProd Nat (Vector F 3))), a = MProd.mk a.1 a.2 := by
+    intro a
+    cases a
+    rfl
+  unfold step_2
+  simp [Id.run]
+  (
+    split
+    rename_i rc sw h
+    have : sw = (MProd.mk rc sw).2 := by rfl
+    rw [this, ←h]
+    clear this rc sw h
+  )
+  (
+    split
+    rename_i rc sw h
+    have : sw = (MProd.mk rc sw).2 := by rfl
+    rw [this, ←h]
+    clear this rc sw h
+  )
+  (
+    split
+    rename_i rc sw h
+    have : sw = (MProd.mk rc sw).2 := by rfl
+    rw [this, ←h]
+    clear this rc sw h
+  )
+  apply congrArg
+  apply congr
+  {
+    apply congrArg
+    rw [this (Poseidon.partial_rounds_step_3 _ _), partial_round_const_count]
+    apply congr
+    {
+      apply congrArg
+      rw [full_round_const_count]
+      simp
+    }
+    {
+      apply congrArg
+      apply congr
+      {
+        apply congrArg
+        rw [this (Poseidon.full_rounds_step_3 _ _), full_round_const_count]
+        rfl
+      }
+      { rfl }
+    }
+  }
+  { rfl }
+
+lemma congrArg2 { a b } {c d} {f : α -> β -> γ }: a = b -> c = d -> f a c = f b d := by
   intros
   congr
 
-lemma mds_uncps (S : Vector F 3) (k : Vector F 3 -> Prop): mds_3 S k = k (mds_matmul S) := by
-  conv => lhs; simp [mds_3, Gates.add, Gates.mul]
+lemma vec_zero_eq (v1 v2 : Vector F 3): v1 = v2 -> v1[0] = v2[0] := by
+  intro h
+  rw [h]
+
+lemma poseidon_uncps (A B : F) (k : F -> Prop): Poseidon A B k = k (Poseidon.perm vec![0, A, B])[0] := by
+  rw [looped_Poseidon'_go, looped_Poseidon', full_rounds_uncps, partial_rounds_uncps, full_rounds_uncps]
+  apply congrArg
+  simp [Poseidon.step1_go, step_2_go, step_2]
+  simp [Id.run]
+  apply vec_zero_eq
+  (
+    split
+    rename_i rc sw h
+    have : sw = (MProd.mk rc sw).2 := by rfl
+    rw [this, ←h]
+    clear this rc sw h
+  )
+  (
+    split
+    rename_i rc sw h
+    have : sw = (MProd.mk rc sw).2 := by rfl
+    rw [this, ←h]
+    clear this rc sw h
+  )
+  (
+    split
+    rename_i rc sw h
+    have : sw = (MProd.mk rc sw).2 := by rfl
+    rw [this, ←h]
+    clear this rc sw h
+  )
   congr
-  simp [mds_matmul, Matrix.mul_apply]
-  repeat (any_goals (apply vec_eq))
-  . simp [Finset.univ, Fintype.elems, mul_comm, add_assoc, Matrix.column_from_vector]
-  . simp [Finset.univ, Fintype.elems, mul_comm, add_assoc, Matrix.column_from_vector]
-  . simp [Finset.univ, Fintype.elems]
-    conv => lhs; simp [mul_comm, add_assoc]
-  . rfl
-
-def full_round (S C: Vector F 3) : Vector F 3 :=
-  mds_matmul vec![(S[0] + C[0]) ^ 5, (S[1] + C[1]) ^ 5, (S[2] + C[2]) ^ 5]
-
-def full_round_with_const (i: Nat) (S : Vector F 3) : Vector F 3 :=
-  let c := vec![Poseidon.round_constants_field[3 * i]!, Poseidon.round_constants_field[3 * i + 1]!, Poseidon.round_constants_field[3 * i + 2]!]
-  full_round S c
-
-lemma full_round_uncps (S C: Vector F 3) (k : Vector F 3 -> Prop): fullRound_3_3 S C k = k (full_round S C) := by
-  conv => lhs; simp [fullRound_3_3, Gates.add, sbox_uncps, mds_uncps]
-
-def half_round (S C: Vector F 3) : Vector F 3 :=
-  mds_matmul vec![(S[0] + C[0]) ^ 5, S[1] + C[1], S[2] + C[2]]
-
-def half_round_with_const(i: Nat) (S : Vector F 3) : Vector F 3 :=
-  let c := vec![Poseidon.round_constants_field[3 * i]!, Poseidon.round_constants_field[3 * i + 1]!, Poseidon.round_constants_field[3 * i + 2]!]
-  half_round S c
-
-lemma half_round_uncps (S C: Vector F 3) (k : Vector F 3 -> Prop): halfRound_3_3 S C k = k (half_round S C) := by
-  conv => lhs; simp [halfRound_3_3, Gates.add, sbox_uncps, mds_uncps]
-
-
-def generic_loop (S : α) (start stop: Nat) (f : Nat -> α -> α) : α := Id.run do
-  let mut state := S
-  for i in [start:stop] do
-    state := f i state
-  state
-
-def generic_recur (S : α) (start stop : Nat) (f : Nat -> α -> α) : α := go stop start stop S where
-  go fuel start stop s := if stop ≤ start then s else match fuel with
-    | Nat.zero => s
-    | Nat.succ fuel => go fuel (start + 1) stop (f start s)
-
--- fuel₀ = stop, start₀ = start
--- fuel₁ = stop - 1, start₁ = start + 1
--- fuel₂ = stop - 2, start₂ = start + 2
--- fuelₙ + startₙ = start + stop
-
-lemma generic_recur_empty (S: α) (start: Nat) (f : Nat -> α -> α):
-  generic_recur S start start f = S := by
-  unfold generic_recur
-  unfold generic_recur.go
-  simp
-
-
-lemma generic_recur_cons (S : α) (start d : Nat) (f : Nat -> α -> α):
-  generic_recur S start (start + d.succ) f = generic_recur  (f start S) (start + 1) (start + d.succ) f := by
-  have : ∀ (S : α) (start fuel1 fuel2 d : Nat) (f : Nat -> α -> α),
-    (fuel1 >= d.succ) ->
-    (fuel2 >= d.succ) ->
-    generic_recur.go f fuel1 start (start + d.succ) S = generic_recur.go f fuel2 (start + 1) (start + d.succ) (f start S) := by
-    intro S start fuel1 fuel2 d f h1 h2
-    induction d generalizing fuel1 fuel2 start S f with
-    | zero =>
-      unfold generic_recur.go
-      simp
-      split
-      . contradiction
-      . unfold generic_recur.go; simp
-    | succ d ih =>
-      unfold generic_recur.go
-      simp
-      cases fuel1
-      {contradiction}
-      cases fuel2
-      {contradiction}
-      simp
-      split
-      {contradiction}
-      simp
-      conv => lhs; arg 4; rw [Nat.add_succ, ←Nat.succ_add, Nat.add_one, ←Nat.add_one]
-      rw [ih]
-      conv => rhs; arg 4; rw [Nat.add_succ, ←Nat.succ_add, Nat.add_one, ←Nat.add_one]
-      all_goals linarith
-
-  unfold generic_recur
-  conv => lhs; arg 2; rw [Nat.add_succ]
-  rw [this] <;> simp_arith
-
-lemma generic_recur_snoc (S: α) (start d: Nat) (f: Nat -> α -> α):
-  generic_recur S start (start + d.succ) f = f (start + d) (generic_recur S start (start + d) f) := by
-  have go_snoc : ∀ fuel start d s,
-    fuel > d ->
-    generic_recur.go f fuel start (start + d.succ) s = f (start + d) (generic_recur.go f (fuel - 1) start (start + d) s) := by
-    intro fuel start d s
-    induction d generalizing fuel start s with
-    | zero =>
-      intro h
-      unfold generic_recur.go
-      simp
-      split
-      . contradiction
-      . simp
-        unfold generic_recur.go
-        simp
-    | succ d ih =>
-      intro h
-      conv => lhs ; unfold generic_recur.go ; simp
-      cases fuel
-      . contradiction
-      . rename_i fuelᵢ
-        simp
-        conv =>
-          lhs
-          arg 4
-          rw [Nat.add_succ, ←Nat.succ_add, Nat.add_one]
-          arg 1
-          rw [←Nat.add_one]
-        rw [ih]
-        . conv => lhs; arg 1; rw [Nat.add_assoc]; rw [Nat.one_add]
-          apply congrArg
-          conv =>
-            rhs
-            unfold generic_recur.go
-            simp
-          cases fuelᵢ
-          . contradiction
-          . simp
-            conv => lhs; arg 4; rw [Nat.add_assoc]; rw [Nat.one_add]
-        . linarith
-
-  unfold generic_recur
-  apply go_snoc
-  linarith
-
-
-
-def generic_recur_non_tail (S : α) (start stop : Nat) (f : Nat -> α -> α): α := go stop start stop S where
-  go fuel start stop s := if stop ≤ start then s else match fuel with
-    | Nat.zero => s
-    | Nat.succ fuel => f (stop - 1)  (go fuel start (stop - 1) s)
-
-lemma generic_recur_tail_non_tail (S: α) (start d : Nat) (f : Nat -> α -> α) :
-  generic_recur S start (start + d) f = generic_recur_non_tail S start (start + d) f := by
-  have : ∀ fuel start stop s, generic_recur.go f fuel start stop s = generic_recur_non_tail.go f fuel start stop s := by
-    intro fuel start stop s
-    induction fuel generalizing start stop s with
-    | zero => rfl
-    | succ fuel ih =>
-      unfold generic_recur.go
-      split
-      . sorry
-      . sorry
-      -- unfold generic_recur_non_tail.go
-      -- split_ifs
-      -- . rfl
-      -- . simp
-      --   rw [ih]
-  induction d with
-  | zero =>
-    simp [generic_recur, generic_recur_non_tail]
-    unfold generic_recur.go
-    unfold generic_recur_non_tail.go
-    simp
-  | succ d ih =>
-    simp [generic_recur, generic_recur_non_tail]
-    unfold generic_recur.go
-    unfold generic_recur_non_tail.go
-    simp
-    sorry
-
-
-theorem generic_loop_or_recur (S : α) (start stop: Nat) (f : Nat -> α -> α) : generic_loop S start stop f = generic_recur S start stop f := by
-  have inside : ∀ s (fuel start stop : Nat),
-    generic_recur.go f fuel start stop s =
-    Id.run (Std.Range.forIn.loop (fun i x => pure (ForInStep.yield (f i x))) fuel start stop 1 s) := by
-      intros s fuel start stop
-      simp [Id.run]
-      induction fuel generalizing start s with
-      | zero =>
-        simp [generic_recur.go, Std.Range.forIn.loop]
-      | succ fuel ih =>
-        simp [generic_recur.go, Std.Range.forIn.loop]
-        split_ifs
-        . rfl
-        . apply ih
-  simp [generic_loop, generic_recur, Id.run, forIn, Std.Range.forIn, inside]
-
-def full_rounds_loop (S : Vector F 3) (start stop : Nat) : Vector F 3 := Id.run do
-  let mut state := S
-  for i in [start:stop] do
-    state := full_round_with_const i state
-  state
-
-def round_constants' (i : Nat) : Vector F 3 := vec![Poseidon.round_constants_field[3 * i]!, Poseidon.round_constants_field[3 * i + 1]!, Poseidon.round_constants_field[3 * i + 2]!]
-
-def full_rounds_no_loop (S : Vector F 3) (start stop : Nat) : Vector F 3 := generic_recur S start stop fun i S =>
-  full_round S vec![Poseidon.round_constants_field[3 * i]!, Poseidon.round_constants_field[3 * i + 1]!, Poseidon.round_constants_field[3 * i + 2]!]
-
-lemma full_rounds_loop_generic S start stop : full_rounds_loop S start stop = generic_loop S start stop full_round_with_const := by
-  simp [full_rounds_loop, generic_loop, full_round_with_const]
-
-lemma full_rounds_no_loop_generic S start stop : full_rounds_no_loop S start stop = generic_recur S start stop full_round_with_const := by
-  simp [full_rounds_no_loop, generic_recur, full_round_with_const]
-
-lemma full_rounds_loop_recur {S : Vector F 3} {start count : Nat} : full_rounds_loop S start count = full_rounds_no_loop S start count := by
-  rw [full_rounds_loop_generic, full_rounds_no_loop_generic, generic_loop_or_recur]
-
-def half_rounds_loop (S : Vector F 3) (start stop : Nat) : Vector F 3 := Id.run do
-  let mut state := S
-  for i in [start:stop] do
-    state := half_round_with_const i state
-  state
-
-def half_rounds_no_loop (S : Vector F 3) (start stop : Nat) : Vector F 3 := generic_recur S start stop fun i S =>
-  half_round S vec![Poseidon.round_constants_field[3 * i]!, Poseidon.round_constants_field[3 * i + 1]!, Poseidon.round_constants_field[3 * i + 2]!]
-
-lemma half_rounds_loop_generic S start stop : half_rounds_loop S start stop = generic_loop S start stop half_round_with_const := by
-  simp [half_rounds_loop, generic_loop, half_round_with_const]
-
-lemma half_rounds_no_loop_generic S start stop : half_rounds_no_loop S start stop = generic_recur S start stop half_round_with_const := by
-  simp [half_rounds_no_loop, generic_recur, half_round_with_const]
-
-lemma half_rounds_loop_recur (S : Vector F 3) (start count : Nat) : half_rounds_loop S start count = half_rounds_no_loop S start count := by
-  rw [half_rounds_loop_generic, half_rounds_no_loop_generic, generic_loop_or_recur]
-
-def poseidon_looped_fnd (S : Vector F 3): Vector F 3 := Id.run do
-  let mut state := S
-  state := full_rounds_loop state 0 4
-  state := half_rounds_loop state 4 61
-  state := full_rounds_loop state 61 65
-  state
-
-def poseidon_non_looped (S : Vector F 3): Vector F 3 := Id.run do
-  let mut state := S
-  state := full_rounds_no_loop state 0 4
-  state := half_rounds_no_loop state 4 61
-  state := full_rounds_no_loop state 61 65
-  state
-
-def poseidon_looped (S : Vector F 3): Vector F 3 := Id.run do
-  let mut state := S
-  for i in [0:4] do
-    let c := vec![Poseidon.round_constants_field[3 * i]!, Poseidon.round_constants_field[3 * i + 1]!, Poseidon.round_constants_field[3 * i + 2]!]
-    state := full_round state c
-  for i in [4:61] do
-    let c := vec![Poseidon.round_constants_field[3 * i]!, Poseidon.round_constants_field[3 * i + 1]!, Poseidon.round_constants_field[3 * i + 2]!]
-    state := half_round state c
-  for i in [61:65] do
-    let c := vec![Poseidon.round_constants_field[3 * i]!, Poseidon.round_constants_field[3 * i + 1]!, Poseidon.round_constants_field[3 * i + 2]!]
-    state := full_round state c
-  state
-
-theorem unIdRun (x : Id α) : Id.run x = x := by
-  simp [Id.run]
-
-theorem poseidon_looped_unfndd S : poseidon_looped_fnd S = poseidon_looped S := by
-  simp [
-    poseidon_looped_fnd,
-    poseidon_looped,
-    full_rounds_loop,
-    half_rounds_loop,
-    full_round_with_const,
-    half_round_with_const,
-    unIdRun
-  ]
-
-lemma poseidon_looped_non_looped (S : Vector F 3): poseidon_looped S = poseidon_non_looped S := by
-  rw [←poseidon_looped_unfndd, poseidon_looped_fnd]
-  simp [unIdRun]
-  rw [full_rounds_loop_recur, half_rounds_loop_recur, full_rounds_loop_recur]
-  sorry
-  -- rw
-
-
--- set_option maxRecDepth 1024
--- set_option maxHeartbeats 0
-
-lemma vecEqs (v₁ v₂ : Vector α 3) : v₁ = v₂ -> v₁[0] = v₂[0] := by intros; congr
-
-lemma congrArg2 {a b : α} { c d : β } {f : α -> β -> γ } : a = b -> c = d -> f a c = f b d :=
-  by intros; congr
-
--- set_option maxRecDepth 1024
-
-def zipfold (f : α -> β -> α) (init : α) (params : Vector β len) := match len with
-  | Nat.zero => init
-  | Nat.succ _ => zipfold f (f init params.head) params.tail
-
-def poseidon_constants_rounds (start d : Nat) : Vector (Vector F 3) d := match d with
-  | Nat.zero => Vector.nil
-  | Nat.succ d => (poseidon_constants_rounds start d).snoc (round_constants' (start + d))
-
--- theorem full_rounds_no_loop_zipfold (start d : Nat) : full_rounds_no_loop ()
-
-lemma zipfold_1 (f : α -> β -> α) (init : α) (param : β) : f init param = zipfold f init vec![param] := by
-  simp [zipfold]
-
-lemma zipfold_next (f : α -> β -> α) (init: α) (param : β) (params : Vector β len) : zipfold f (f init param) params = zipfold f init (param ::ᵥ params) := by
-  simp [zipfold]
-
-lemma zipfold_snoc (f : α -> β -> α) (init: α) (param : β) (params : Vector β len) : zipfold f init (params.snoc param) = f (zipfold f init params) param := by
-  induction len generalizing init with
-  | zero =>
-    simp [zipfold, Vector.eq_nil]
-  | succ len ih =>
-    conv =>
-      lhs
-      unfold zipfold
-      rw [Vector.tail_snoc, Vector.head_snoc, ih]
-
-
-def full_rounds_zipfold (start len : Nat) (inp : Vector F 3): Vector F 3 :=
-  zipfold full_round inp (poseidon_constants_rounds start len)
-
-lemma full_rounds_recur_zipfold {start len : Nat} {inp : Vector F 3}:
-  full_rounds_zipfold start len inp = full_rounds_no_loop inp start (start + len) := by
-  induction len generalizing inp with
-  | zero =>
-    simp [full_rounds_zipfold, full_rounds_no_loop, generic_recur_empty, poseidon_constants_rounds, zipfold]
-  | succ len ih =>
-    simp [full_rounds_zipfold, full_rounds_no_loop] at ih
-    simp [full_rounds_zipfold, poseidon_constants_rounds, zipfold_snoc, round_constants']
-    simp [full_rounds_no_loop, generic_recur_snoc]
-    congr
-    apply ih
-
--- set_option maxRecDepth 4096
--- set_option maxHeartbeats 0
-
-lemma half_rounds_recur_zipfold {start len : Nat} {inp : Vector F 3}:
-  zipfold half_round inp (poseidon_constants_rounds start len) = half_rounds_no_loop inp start (start + len) := by
-  induction len generalizing inp with
-  | zero =>
-    simp [half_rounds_no_loop, generic_recur_empty, poseidon_constants_rounds, zipfold]
-  | succ len ih =>
-    simp [half_rounds_no_loop] at ih
-    simp [poseidon_constants_rounds, zipfold_snoc, round_constants']
-    simp [half_rounds_no_loop, generic_recur_snoc]
-    congr
-    apply ih
-
-lemma iff_reverse (v1 v2 : Vector α len): v1 = v2 ↔ v1.reverse = v2.reverse := by sorry
-
-lemma vec_get_list {v : Vector α len} {i : Nat} { _ : i < len } : v[i] = v.toList.get ⟨i, by rw [Vector.toList_length]; assumption⟩  := by
-  simp [getElem!, getElem, List.get]
-
-lemma iff_to_eq (a b : α) (k : α -> Prop): a = b -> (k a ↔ k b) := by intro hp; rw [hp]
-
-set_option maxHeartbeats 0
-set_option maxRecDepth 1024
-
-                      -- (forIn { start := 0, stop := 3, step := 1 } state_words fun i r =>
-                      --   ForInStep.yield (Vector.set r (↑i) (r[i]! ^ 5)))))
-
-lemma lemma1 {state_words : Vector F 3}:
-  (forIn (m := Id) [0:3] state_words fun (i:Nat) r => ForInStep.yield (Vector.set r i (r[i]! ^ 5)))
-  = vec![state_words[0]! ^ 5, state_words[1]! ^ 5, state_words[2]! ^ 5] := by
-  sorry
-
-lemma looped_poseidon_correct {inp : Vector F 3}: poseidon_looped inp = Poseidon.perm inp := by
-  simp [Poseidon.perm, Poseidon.R_F, Poseidon.t]
-  simp [Id.run]
-  split
-
-
---   rw [unIdRun]
---   split
-
-
--- THIS ALSO WORKS
-
--- lemma poseidon_uncps (A B : F) (k : F -> Prop): Poseidon A B k = k (poseidon_looped vec![0, A, B])[0] := by
---   simp [Poseidon, full_round_uncps, half_round_uncps]
---   apply iff_to_eq
---   apply Vector.head_eq
---   simp [poseidon_looped_non_looped, poseidon_non_looped, unIdRun]
---   repeat (apply congrArg2)
---   all_goals rfl
-
-
-
-
-
--- THIS WORKS
-
--- lemma poseidon_uncps (A B : F) (k : F -> Prop): Poseidon A B k = k (poseidon_looped vec![0, A, B])[0] := by
---   simp [Poseidon, full_round_uncps, half_round_uncps]
---   apply iff_to_eq
---   apply Vector.head_eq
---   rw [zipfold_1 full_round _ _]
---   repeat (rw [zipfold_next full_round _ _])
---   rw [zipfold_1 half_round]
---   repeat (rw [zipfold_next half_round])
---   rw [zipfold_1 full_round]
---   repeat (rw [zipfold_next full_round])
---   rw [poseidon_looped_non_looped]
---   simp [poseidon_non_looped, unIdRun]
---   have : 65 = 61 + 4 := by rfl
---   rw [this, ←full_rounds_recur_zipfold]
---   rw [full_rounds_zipfold]
---   apply congr
---   apply congr
---   { rfl }
---   have : 61 = 4 + 57 := by rfl
---   rw [this, ←half_rounds_recur_zipfold]
---   apply congr
---   apply congr
---   { rfl }
---   have : 4 = 0 + 4 := by rfl
---   rw [this]
---   rw [←full_rounds_recur_zipfold]
---   rw [full_rounds_zipfold]
---   apply congr
---   {rfl}
---   {
---     rfl
---   }
---   {
---     simp [poseidon_constants_rounds]
---     rw [iff_reverse]
---     repeat (rw [Vector.reverse_snoc_cons])
---     rw [Vector.reverse_singleton]
---     apply Vector.eq
---     rw [Vector.toList_reverse]
---     simp
---     repeat (apply And.intro; swap)
---     all_goals rfl
---   }
---   {
---     rfl
---   }
-
-
-
---- END WORKS
-
-
-  -- apply vecEqs
-  -- simp [
-  --   poseidon_looped_non_looped,
-  --   poseidon_non_looped,
-  --   unIdRun
-  -- ]
-  -- simp [full_rounds_no_loop]
-  -- have : 65 = 61 + 4 := by rfl
-  -- simp [this, generic_recur_snoc, generic_recur_empty]
-  -- apply congrArg2; rotate_left; unfold Poseidon.round_constants_field; simp_arith;
-
-
-  -- have : 4 = 0 + 4 := by rfl
-  -- conv in generic_recur _ 0 4 _ => simp [this]
-  -- -- simp [this]
-  -- have : 65 = 61 + 4 := by rfl
-
-  -- simp [generic_recur_snoc, generic_recur_empty]
-
-
-
-
-
-
-    -- simp [poseidon_looped_non_looped, poseidon_non_looped, unIdRun, full_rounds_no_loop, half_rounds_no_loop]
-
-
-
---   simp_arith
---   rfl
-
-  -- conv =>
-  --   lhs
-  --   arg 2
-
-  -- congr
-
-  -- apply congrArg
-  -- simp [sbox, Gates.mul]
-  -- conv in (_ ^ _) => whnf
-  -- rfl
-
-
--- lemma looped_correct (A B : F) (k : F -> Prop): looped_Poseidon A B k ↔ k (Poseidon.perm #[0, A, B])[0]! := by
---   unfold looped_Poseidon
---   unfold Poseidon.perm
---   simp [Id.run, forIn, Std.Range.forIn, Poseidon.R_F]
---   unfold Std.Range.forIn.loop
-
---   sorry
