ProvenZk/PoseidonCorrectness2.lean
@@ -1,0 +1,509 @@
+import ProvenZk.PoseidonExtract
+import ProvenZk.Poseidon
+import ProvenZk.VectorExtensions
+-- import Mathlib
+
+variable [Fact (Nat.Prime Order)]
+
+lemma fin_mod { n } (x : Fin n) : x.val = x.val % n := by
+  have : _ := x.isLt
+  simp [Nat.mod_eq_of_lt this]
+
+
+-- def foo :=   [0:10].forIn
+lemma sbox_uncps (A : F) (k : F -> Prop): sbox A k = k (A ^ 5) := by
+  unfold sbox
+  conv => lhs; simp [Gates.mul]
+  apply congrArg
+  rw [mul_assoc]
+  conv => rhs; whnf
+  conv => lhs; whnf
+  congr
+  simp_arith
+  apply fin_mod _
+
+def mds_matmul (S : Vector F 3) : Vector F 3 :=
+  let smat := Matrix.column_from_vector S
+  let rmat := Poseidon.MDS_matrix_field.mul smat
+  vec![rmat 0 0, rmat 1 0, rmat 2 0]
+
+lemma vec_eq (a b : α) (t s : Vector α n) : a = b -> t = s -> a ::ᵥ t = b ::ᵥ s := by
+  intros
+  congr
+
+lemma mds_uncps (S : Vector F 3) (k : Vector F 3 -> Prop): mds_3 S k = k (mds_matmul S) := by
+  conv => lhs; simp [mds_3, Gates.add, Gates.mul]
+  congr
+  simp [mds_matmul, Matrix.mul_apply]
+  repeat (any_goals (apply vec_eq))
+  . simp [Finset.univ, Fintype.elems, mul_comm, add_assoc, Matrix.column_from_vector]
+  . simp [Finset.univ, Fintype.elems, mul_comm, add_assoc, Matrix.column_from_vector]
+  . simp [Finset.univ, Fintype.elems]
+    conv => lhs; simp [mul_comm, add_assoc]
+  . rfl
+
+def full_round (S C: Vector F 3) : Vector F 3 :=
+  mds_matmul vec![(S[0] + C[0]) ^ 5, (S[1] + C[1]) ^ 5, (S[2] + C[2]) ^ 5]
+
+def full_round_with_const (i: Nat) (S : Vector F 3) : Vector F 3 :=
+  let c := vec![Poseidon.round_constants_field[3 * i]!, Poseidon.round_constants_field[3 * i + 1]!, Poseidon.round_constants_field[3 * i + 2]!]
+  full_round S c
+
+lemma full_round_uncps (S C: Vector F 3) (k : Vector F 3 -> Prop): fullRound_3_3 S C k = k (full_round S C) := by
+  conv => lhs; simp [fullRound_3_3, Gates.add, sbox_uncps, mds_uncps]
+
+def half_round (S C: Vector F 3) : Vector F 3 :=
+  mds_matmul vec![(S[0] + C[0]) ^ 5, S[1] + C[1], S[2] + C[2]]
+
+def half_round_with_const(i: Nat) (S : Vector F 3) : Vector F 3 :=
+  let c := vec![Poseidon.round_constants_field[3 * i]!, Poseidon.round_constants_field[3 * i + 1]!, Poseidon.round_constants_field[3 * i + 2]!]
+  half_round S c
+
+lemma half_round_uncps (S C: Vector F 3) (k : Vector F 3 -> Prop): halfRound_3_3 S C k = k (half_round S C) := by
+  conv => lhs; simp [halfRound_3_3, Gates.add, sbox_uncps, mds_uncps]
+
+
+def generic_loop (S : α) (start stop: Nat) (f : Nat -> α -> α) : α := Id.run do
+  let mut state := S
+  for i in [start:stop] do
+    state := f i state
+  state
+
+def generic_recur (S : α) (start stop : Nat) (f : Nat -> α -> α) : α := go stop start stop S where
+  go fuel start stop s := if stop ≤ start then s else match fuel with
+    | Nat.zero => s
+    | Nat.succ fuel => go fuel (start + 1) stop (f start s)
+
+-- fuel₀ = stop, start₀ = start
+-- fuel₁ = stop - 1, start₁ = start + 1
+-- fuel₂ = stop - 2, start₂ = start + 2
+-- fuelₙ + startₙ = start + stop
+
+lemma generic_recur_empty (S: α) (start: Nat) (f : Nat -> α -> α):
+  generic_recur S start start f = S := by
+  unfold generic_recur
+  unfold generic_recur.go
+  simp
+
+
+lemma generic_recur_cons (S : α) (start d : Nat) (f : Nat -> α -> α):
+  generic_recur S start (start + d.succ) f = generic_recur  (f start S) (start + 1) (start + d.succ) f := by
+  have : ∀ (S : α) (start fuel1 fuel2 d : Nat) (f : Nat -> α -> α),
+    (fuel1 >= d.succ) ->
+    (fuel2 >= d.succ) ->
+    generic_recur.go f fuel1 start (start + d.succ) S = generic_recur.go f fuel2 (start + 1) (start + d.succ) (f start S) := by
+    intro S start fuel1 fuel2 d f h1 h2
+    induction d generalizing fuel1 fuel2 start S f with
+    | zero =>
+      unfold generic_recur.go
+      simp
+      split
+      . contradiction
+      . unfold generic_recur.go; simp
+    | succ d ih =>
+      unfold generic_recur.go
+      simp
+      cases fuel1
+      {contradiction}
+      cases fuel2
+      {contradiction}
+      simp
+      split
+      {contradiction}
+      simp
+      conv => lhs; arg 4; rw [Nat.add_succ, ←Nat.succ_add, Nat.add_one, ←Nat.add_one]
+      rw [ih]
+      conv => rhs; arg 4; rw [Nat.add_succ, ←Nat.succ_add, Nat.add_one, ←Nat.add_one]
+      all_goals linarith
+
+  unfold generic_recur
+  conv => lhs; arg 2; rw [Nat.add_succ]
+  rw [this] <;> simp_arith
+
+lemma generic_recur_snoc (S: α) (start d: Nat) (f: Nat -> α -> α):
+  generic_recur S start (start + d.succ) f = f (start + d) (generic_recur S start (start + d) f) := by
+  have go_snoc : ∀ fuel start d s,
+    fuel > d ->
+    generic_recur.go f fuel start (start + d.succ) s = f (start + d) (generic_recur.go f (fuel - 1) start (start + d) s) := by
+    intro fuel start d s
+    induction d generalizing fuel start s with
+    | zero =>
+      intro h
+      unfold generic_recur.go
+      simp
+      split
+      . contradiction
+      . simp
+        unfold generic_recur.go
+        simp
+    | succ d ih =>
+      intro h
+      conv => lhs ; unfold generic_recur.go ; simp
+      cases fuel
+      . contradiction
+      . rename_i fuelᵢ
+        simp
+        conv =>
+          lhs
+          arg 4
+          rw [Nat.add_succ, ←Nat.succ_add, Nat.add_one]
+          arg 1
+          rw [←Nat.add_one]
+        rw [ih]
+        . conv => lhs; arg 1; rw [Nat.add_assoc]; rw [Nat.one_add]
+          apply congrArg
+          conv =>
+            rhs
+            unfold generic_recur.go
+            simp
+          cases fuelᵢ
+          . contradiction
+          . simp
+            conv => lhs; arg 4; rw [Nat.add_assoc]; rw [Nat.one_add]
+        . linarith
+
+  unfold generic_recur
+  apply go_snoc
+  linarith
+
+
+
+def generic_recur_non_tail (S : α) (start stop : Nat) (f : Nat -> α -> α): α := go stop start stop S where
+  go fuel start stop s := if stop ≤ start then s else match fuel with
+    | Nat.zero => s
+    | Nat.succ fuel => f (stop - 1)  (go fuel start (stop - 1) s)
+
+lemma generic_recur_tail_non_tail (S: α) (start d : Nat) (f : Nat -> α -> α) :
+  generic_recur S start (start + d) f = generic_recur_non_tail S start (start + d) f := by
+  have : ∀ fuel start stop s, generic_recur.go f fuel start stop s = generic_recur_non_tail.go f fuel start stop s := by
+    intro fuel start stop s
+    induction fuel generalizing start stop s with
+    | zero => rfl
+    | succ fuel ih =>
+      unfold generic_recur.go
+      split
+      . sorry
+      . sorry
+      -- unfold generic_recur_non_tail.go
+      -- split_ifs
+      -- . rfl
+      -- . simp
+      --   rw [ih]
+  induction d with
+  | zero =>
+    simp [generic_recur, generic_recur_non_tail]
+    unfold generic_recur.go
+    unfold generic_recur_non_tail.go
+    simp
+  | succ d ih =>
+    simp [generic_recur, generic_recur_non_tail]
+    unfold generic_recur.go
+    unfold generic_recur_non_tail.go
+    simp
+    sorry
+
+
+theorem generic_loop_or_recur (S : α) (start stop: Nat) (f : Nat -> α -> α) : generic_loop S start stop f = generic_recur S start stop f := by
+  have inside : ∀ s (fuel start stop : Nat),
+    generic_recur.go f fuel start stop s =
+    Id.run (Std.Range.forIn.loop (fun i x => pure (ForInStep.yield (f i x))) fuel start stop 1 s) := by
+      intros s fuel start stop
+      simp [Id.run]
+      induction fuel generalizing start s with
+      | zero =>
+        simp [generic_recur.go, Std.Range.forIn.loop]
+      | succ fuel ih =>
+        simp [generic_recur.go, Std.Range.forIn.loop]
+        split_ifs
+        . rfl
+        . apply ih
+  simp [generic_loop, generic_recur, Id.run, forIn, Std.Range.forIn, inside]
+
+def full_rounds_loop (S : Vector F 3) (start stop : Nat) : Vector F 3 := Id.run do
+  let mut state := S
+  for i in [start:stop] do
+    state := full_round_with_const i state
+  state
+
+def round_constants' (i : Nat) : Vector F 3 := vec![Poseidon.round_constants_field[3 * i]!, Poseidon.round_constants_field[3 * i + 1]!, Poseidon.round_constants_field[3 * i + 2]!]
+
+def full_rounds_no_loop (S : Vector F 3) (start stop : Nat) : Vector F 3 := generic_recur S start stop fun i S =>
+  full_round S vec![Poseidon.round_constants_field[3 * i]!, Poseidon.round_constants_field[3 * i + 1]!, Poseidon.round_constants_field[3 * i + 2]!]
+
+lemma full_rounds_loop_generic S start stop : full_rounds_loop S start stop = generic_loop S start stop full_round_with_const := by
+  simp [full_rounds_loop, generic_loop, full_round_with_const]
+
+lemma full_rounds_no_loop_generic S start stop : full_rounds_no_loop S start stop = generic_recur S start stop full_round_with_const := by
+  simp [full_rounds_no_loop, generic_recur, full_round_with_const]
+
+lemma full_rounds_loop_recur {S : Vector F 3} {start count : Nat} : full_rounds_loop S start count = full_rounds_no_loop S start count := by
+  rw [full_rounds_loop_generic, full_rounds_no_loop_generic, generic_loop_or_recur]
+
+def half_rounds_loop (S : Vector F 3) (start stop : Nat) : Vector F 3 := Id.run do
+  let mut state := S
+  for i in [start:stop] do
+    state := half_round_with_const i state
+  state
+
+def half_rounds_no_loop (S : Vector F 3) (start stop : Nat) : Vector F 3 := generic_recur S start stop fun i S =>
+  half_round S vec![Poseidon.round_constants_field[3 * i]!, Poseidon.round_constants_field[3 * i + 1]!, Poseidon.round_constants_field[3 * i + 2]!]
+
+lemma half_rounds_loop_generic S start stop : half_rounds_loop S start stop = generic_loop S start stop half_round_with_const := by
+  simp [half_rounds_loop, generic_loop, half_round_with_const]
+
+lemma half_rounds_no_loop_generic S start stop : half_rounds_no_loop S start stop = generic_recur S start stop half_round_with_const := by
+  simp [half_rounds_no_loop, generic_recur, half_round_with_const]
+
+lemma half_rounds_loop_recur (S : Vector F 3) (start count : Nat) : half_rounds_loop S start count = half_rounds_no_loop S start count := by
+  rw [half_rounds_loop_generic, half_rounds_no_loop_generic, generic_loop_or_recur]
+
+def poseidon_looped_fnd (S : Vector F 3): Vector F 3 := Id.run do
+  let mut state := S
+  state := full_rounds_loop state 0 4
+  state := half_rounds_loop state 4 61
+  state := full_rounds_loop state 61 65
+  state
+
+def poseidon_non_looped (S : Vector F 3): Vector F 3 := Id.run do
+  let mut state := S
+  state := full_rounds_no_loop state 0 4
+  state := half_rounds_no_loop state 4 61
+  state := full_rounds_no_loop state 61 65
+  state
+
+def poseidon_looped (S : Vector F 3): Vector F 3 := Id.run do
+  let mut state := S
+  for i in [0:4] do
+    let c := vec![Poseidon.round_constants_field[3 * i]!, Poseidon.round_constants_field[3 * i + 1]!, Poseidon.round_constants_field[3 * i + 2]!]
+    state := full_round state c
+  for i in [4:61] do
+    let c := vec![Poseidon.round_constants_field[3 * i]!, Poseidon.round_constants_field[3 * i + 1]!, Poseidon.round_constants_field[3 * i + 2]!]
+    state := half_round state c
+  for i in [61:65] do
+    let c := vec![Poseidon.round_constants_field[3 * i]!, Poseidon.round_constants_field[3 * i + 1]!, Poseidon.round_constants_field[3 * i + 2]!]
+    state := full_round state c
+  state
+
+theorem unIdRun (x : Id α) : Id.run x = x := by
+  simp [Id.run]
+
+theorem poseidon_looped_unfndd S : poseidon_looped_fnd S = poseidon_looped S := by
+  simp [
+    poseidon_looped_fnd,
+    poseidon_looped,
+    full_rounds_loop,
+    half_rounds_loop,
+    full_round_with_const,
+    half_round_with_const,
+    unIdRun
+  ]
+
+lemma poseidon_looped_non_looped (S : Vector F 3): poseidon_looped S = poseidon_non_looped S := by
+  rw [←poseidon_looped_unfndd, poseidon_looped_fnd]
+  simp [unIdRun]
+  rw [full_rounds_loop_recur, half_rounds_loop_recur, full_rounds_loop_recur]
+  sorry
+  -- rw
+
+
+-- set_option maxRecDepth 1024
+-- set_option maxHeartbeats 0
+
+lemma vecEqs (v₁ v₂ : Vector α 3) : v₁ = v₂ -> v₁[0] = v₂[0] := by intros; congr
+
+lemma congrArg2 {a b : α} { c d : β } {f : α -> β -> γ } : a = b -> c = d -> f a c = f b d :=
+  by intros; congr
+
+-- set_option maxRecDepth 1024
+
+def zipfold (f : α -> β -> α) (init : α) (params : Vector β len) := match len with
+  | Nat.zero => init
+  | Nat.succ _ => zipfold f (f init params.head) params.tail
+
+def poseidon_constants_rounds (start d : Nat) : Vector (Vector F 3) d := match d with
+  | Nat.zero => Vector.nil
+  | Nat.succ d => (poseidon_constants_rounds start d).snoc (round_constants' (start + d))
+
+-- theorem full_rounds_no_loop_zipfold (start d : Nat) : full_rounds_no_loop ()
+
+lemma zipfold_1 (f : α -> β -> α) (init : α) (param : β) : f init param = zipfold f init vec![param] := by
+  simp [zipfold]
+
+lemma zipfold_next (f : α -> β -> α) (init: α) (param : β) (params : Vector β len) : zipfold f (f init param) params = zipfold f init (param ::ᵥ params) := by
+  simp [zipfold]
+
+lemma zipfold_snoc (f : α -> β -> α) (init: α) (param : β) (params : Vector β len) : zipfold f init (params.snoc param) = f (zipfold f init params) param := by
+  induction len generalizing init with
+  | zero =>
+    simp [zipfold, Vector.eq_nil]
+  | succ len ih =>
+    conv =>
+      lhs
+      unfold zipfold
+      rw [Vector.tail_snoc, Vector.head_snoc, ih]
+
+
+def full_rounds_zipfold (start len : Nat) (inp : Vector F 3): Vector F 3 :=
+  zipfold full_round inp (poseidon_constants_rounds start len)
+
+lemma full_rounds_recur_zipfold {start len : Nat} {inp : Vector F 3}:
+  full_rounds_zipfold start len inp = full_rounds_no_loop inp start (start + len) := by
+  induction len generalizing inp with
+  | zero =>
+    simp [full_rounds_zipfold, full_rounds_no_loop, generic_recur_empty, poseidon_constants_rounds, zipfold]
+  | succ len ih =>
+    simp [full_rounds_zipfold, full_rounds_no_loop] at ih
+    simp [full_rounds_zipfold, poseidon_constants_rounds, zipfold_snoc, round_constants']
+    simp [full_rounds_no_loop, generic_recur_snoc]
+    congr
+    apply ih
+
+-- set_option maxRecDepth 4096
+-- set_option maxHeartbeats 0
+
+lemma half_rounds_recur_zipfold {start len : Nat} {inp : Vector F 3}:
+  zipfold half_round inp (poseidon_constants_rounds start len) = half_rounds_no_loop inp start (start + len) := by
+  induction len generalizing inp with
+  | zero =>
+    simp [half_rounds_no_loop, generic_recur_empty, poseidon_constants_rounds, zipfold]
+  | succ len ih =>
+    simp [half_rounds_no_loop] at ih
+    simp [poseidon_constants_rounds, zipfold_snoc, round_constants']
+    simp [half_rounds_no_loop, generic_recur_snoc]
+    congr
+    apply ih
+
+lemma iff_reverse (v1 v2 : Vector α len): v1 = v2 ↔ v1.reverse = v2.reverse := by sorry
+
+lemma iff_to_eq (a b : α) (k : α -> Prop): a = b -> (k a ↔ k b) := by intro hp; rw [hp]
+
+
+--   rw [unIdRun]
+--   split
+
+
+-- THIS ALSO WORKS
+
+-- set_option maxHeartbeats 1000000
+
+lemma poseidon_uncps (A B : F) (k : F -> Prop): Poseidon A B k = k (Poseidon.perm vec![0, A, B])[0] := by
+  simp [Poseidon, full_round_uncps, half_round_uncps]
+  apply iff_to_eq
+  unfold Poseidon.perm
+  simp [Id.run]
+
+--   simp [Poseidon, full_round_uncps, half_round_uncps]
+--   apply iff_to_eq
+--   apply Vector.head_eq
+--   simp [poseidon_looped_non_looped, poseidon_non_looped, unIdRun]
+--   repeat (apply congrArg2)
+--   all_goals rfl
+
+
+
+
+
+-- THIS WORKS
+
+-- lemma poseidon_uncps (A B : F) (k : F -> Prop): Poseidon A B k = k (poseidon_looped vec![0, A, B])[0] := by
+--   simp [Poseidon, full_round_uncps, half_round_uncps]
+--   apply iff_to_eq
+--   apply Vector.head_eq
+--   rw [zipfold_1 full_round _ _]
+--   repeat (rw [zipfold_next full_round _ _])
+--   rw [zipfold_1 half_round]
+--   repeat (rw [zipfold_next half_round])
+--   rw [zipfold_1 full_round]
+--   repeat (rw [zipfold_next full_round])
+--   rw [poseidon_looped_non_looped]
+--   simp [poseidon_non_looped, unIdRun]
+--   have : 65 = 61 + 4 := by rfl
+--   rw [this, ←full_rounds_recur_zipfold]
+--   rw [full_rounds_zipfold]
+--   apply congr
+--   apply congr
+--   { rfl }
+--   have : 61 = 4 + 57 := by rfl
+--   rw [this, ←half_rounds_recur_zipfold]
+--   apply congr
+--   apply congr
+--   { rfl }
+--   have : 4 = 0 + 4 := by rfl
+--   rw [this]
+--   rw [←full_rounds_recur_zipfold]
+--   rw [full_rounds_zipfold]
+--   apply congr
+--   {rfl}
+--   {
+--     rfl
+--   }
+--   {
+--     simp [poseidon_constants_rounds]
+--     rw [iff_reverse]
+--     repeat (rw [Vector.reverse_snoc_cons])
+--     rw [Vector.reverse_singleton]
+--     apply Vector.eq
+--     rw [Vector.toList_reverse]
+--     simp
+--     repeat (apply And.intro; swap)
+--     all_goals rfl
+--   }
+--   {
+--     rfl
+--   }
+
+
+
+--- END WORKS
+
+
+  -- apply vecEqs
+  -- simp [
+  --   poseidon_looped_non_looped,
+  --   poseidon_non_looped,
+  --   unIdRun
+  -- ]
+  -- simp [full_rounds_no_loop]
+  -- have : 65 = 61 + 4 := by rfl
+  -- simp [this, generic_recur_snoc, generic_recur_empty]
+  -- apply congrArg2; rotate_left; unfold Poseidon.round_constants_field; simp_arith;
+
+
+  -- have : 4 = 0 + 4 := by rfl
+  -- conv in generic_recur _ 0 4 _ => simp [this]
+  -- -- simp [this]
+  -- have : 65 = 61 + 4 := by rfl
+
+  -- simp [generic_recur_snoc, generic_recur_empty]
+
+
+
+
+
+
+    -- simp [poseidon_looped_non_looped, poseidon_non_looped, unIdRun, full_rounds_no_loop, half_rounds_no_loop]
+
+
+
+--   simp_arith
+--   rfl
+
+  -- conv =>
+  --   lhs
+  --   arg 2
+
+  -- congr
+
+  -- apply congrArg
+  -- simp [sbox, Gates.mul]
+  -- conv in (_ ^ _) => whnf
+  -- rfl
+
+
+-- lemma looped_correct (A B : F) (k : F -> Prop): looped_Poseidon A B k ↔ k (Poseidon.perm #[0, A, B])[0]! := by
+--   unfold looped_Poseidon
+--   unfold Poseidon.perm
+--   simp [Id.run, forIn, Std.Range.forIn, Poseidon.R_F]
+--   unfold Std.Range.forIn.loop
+
+--   sorry
